done: modsim -> yord

src/MSim2YOrd.v
@@ -31,13 +31,13 @@ Section PROOF.
 
   Definition lift_wf (wf: WF): WF := sum_WF wf (option_WF wf).
 
-  Definition mk_o (wf: WF) R (o: wf.(T)) (ps: bool) (itr_src: itree srcE R): (lift_wf wf).(T) :=
-    if ps
-    then match (observe itr_src) with
+  Definition mk_o {El Er} (wf: WF) R (o: wf.(T)) (pf: bool) (itr: itree ((El +' cE) +' Er) R): (lift_wf wf).(T) :=
+    if pf
+    then match (observe itr) with
          | VisF ((|Yield)|)%sum _ => (inr (Some o))
          | _ => (inr None)
          end
-    else match (observe itr_src) with
+    else match (observe itr) with
          | VisF ((|Yield)|)%sum _ => (inl o)
          | _ => (inr None)
          end.
@@ -46,6 +46,162 @@ Section PROOF.
   Let wf_ot R0 R1 := @ord_tree_WF (A R0 R1).
   Let wf_stt R0 R1 := lift_wf (@wf_ot R0 R1).
 
+  Lemma modsim_implies_yord
+        tid
+        R0 R1 (LRR: R0 -> R1 -> URA.car -> shared_rel)
+        ps pt r_ctx src tgt
+        (shr: shared)
+        (LSIM: ModSim.lsim I tid LRR ps pt r_ctx src tgt shr)
+    :
+    exists (os ot: (@wf_stt R0 R1).(T)),
+      ModSimYOrd.lsim I wf_stt tid LRR ps pt r_ctx (os, src) (ot, tgt) shr.
+  Proof.
+    eapply modsim_implies_gensim in LSIM. eapply gensim_genos in LSIM. des.
+    exists (mk_o (@wf_ot R0 R1) os pt tgt).
+    exists (mk_o (@wf_ot R0 R1) ot ps src).
+    revert_until tid. ginit. gcofix CIH; i.
+    remember (os, src) as osrc. remember (ot, tgt) as otgt.
+    move LSIM before CIH. revert_until LSIM.
+    pattern R0, R1, LRR, ps, pt, r_ctx, osrc, otgt, shr.
+    revert R0 R1 LRR ps pt r_ctx osrc otgt shr LSIM. apply pind9_acc.
+    intros rr DEC IH. clear DEC. intros R0 R1 LRR ps pt r_ctx osrc otgt shr LSIM.
+    i; clarify.
+    eapply pind9_unfold in LSIM; eauto with paco.
+    inv LSIM.
 
+    { guclo lsim_indC_spec. econs 1; eauto. }
+
+    { destruct GENOS as [GENOS IND]. eapply IH in IND; eauto.
+      guclo lsim_indC_spec. econs 2; eauto.
+      guclo lsim_ord_weakRC_spec. econs; eauto.
+      clear. unfold mk_o. des_ifs; try reflexivity.
+      - right. ss. do 2 econs.
+      - right. ss. do 2 econs.
+    }
+    { des. destruct GENOS as [GENOS IND]. eapply IH in IND; eauto.
+      guclo lsim_indC_spec. econs 3; eauto. exists x.
+      guclo lsim_ord_weakRC_spec. econs; eauto.
+      clear. unfold mk_o. des_ifs; try reflexivity.
+      - right. ss. do 2 econs.
+      - right. ss. do 2 econs.
+    }
+    { destruct GENOS as [GENOS IND]. eapply IH in IND; eauto.
+      guclo lsim_indC_spec. econs 4; eauto.
+      guclo lsim_ord_weakRC_spec. econs; eauto.
+      clear. unfold mk_o. des_ifs; try reflexivity.
+      - right. ss. do 2 econs.
+      - right. ss. do 2 econs.
+    }
+    { destruct GENOS as [GENOS IND]. eapply IH in IND; eauto.
+      guclo lsim_indC_spec. econs 5; eauto.
+      guclo lsim_ord_weakRC_spec. econs; eauto.
+      clear. unfold mk_o. des_ifs; try reflexivity.
+      - right. ss. do 2 econs.
+      - right. ss. do 2 econs.
+    }
+    { destruct GENOS as [GENOS IND]. eapply IH in IND; eauto.
+      guclo lsim_indC_spec. econs 6; eauto.
+      guclo lsim_ord_weakRC_spec. econs; eauto.
+      clear. unfold mk_o. des_ifs; try reflexivity.
+      - right. ss. do 2 econs.
+      - right. ss. do 2 econs.
+    }
+    { guclo lsim_indC_spec. econs 7; eauto. }
+    { des. destruct GENOS0 as [GENOS IND]. eapply IH in IND; eauto.
+      guclo lsim_indC_spec. econs 8; eauto. esplits; eauto.
+      guclo lsim_ord_weakRC_spec. econs; eauto.
+      clear. unfold mk_o. des_ifs; try reflexivity.
+      - right. ss. do 2 econs.
+      - right. ss. do 2 econs.
+    }
+
+    { destruct GENOS as [GENOS IND]. eapply IH in IND; eauto.
+      guclo lsim_indC_spec. econs 9; eauto.
+      guclo lsim_ord_weakLC_spec. econs; eauto.
+      clear. unfold mk_o. des_ifs; try reflexivity.
+      - right. ss. do 2 econs.
+      - right. ss. do 2 econs.
+    }
+    { guclo lsim_indC_spec. econs 10; eauto. i. specialize (GENOS x).
+      destruct GENOS as [GENOS IND]. eapply IH in IND; eauto.
+      guclo lsim_ord_weakLC_spec. econs; eauto.
+      clear. unfold mk_o. des_ifs; try reflexivity.
+      - right. ss. do 2 econs.
+      - right. ss. do 2 econs.
+    }
+    { destruct GENOS as [GENOS IND]. eapply IH in IND; eauto.
+      guclo lsim_indC_spec. econs 11; eauto.
+      guclo lsim_ord_weakLC_spec. econs; eauto.
+      clear. unfold mk_o. des_ifs; try reflexivity.
+      - right. ss. do 2 econs.
+      - right. ss. do 2 econs.
+    }
+    { destruct GENOS as [GENOS IND]. eapply IH in IND; eauto.
+      guclo lsim_indC_spec. econs 12; eauto.
+      guclo lsim_ord_weakLC_spec. econs; eauto.
+      clear. unfold mk_o. des_ifs; try reflexivity.
+      - right. ss. do 2 econs.
+      - right. ss. do 2 econs.
+    }
+    { destruct GENOS as [GENOS IND]. eapply IH in IND; eauto.
+      guclo lsim_indC_spec. econs 13; eauto.
+      guclo lsim_ord_weakLC_spec. econs; eauto.
+      clear. unfold mk_o. des_ifs; try reflexivity.
+      - right. ss. do 2 econs.
+      - right. ss. do 2 econs.
+    }
+    { guclo lsim_indC_spec. econs 14; eauto. i. specialize (GENOS _ FAIR).
+      destruct GENOS as [GENOS IND]. eapply IH in IND; eauto.
+      guclo lsim_ord_weakLC_spec. econs; eauto.
+      clear. unfold mk_o. des_ifs; try reflexivity.
+      - right. ss. do 2 econs.
+      - right. ss. do 2 econs.
+    }
+
+    { guclo lsim_indC_spec. econs 15; eauto. i. specialize (GENOS ret).
+      destruct GENOS as [GENOS IND]. eapply IH in IND; eauto.
+      guclo lsim_ord_weakLC_spec. econs; eauto.
+      guclo lsim_ord_weakRC_spec. econs; eauto.
+      - clear. unfold mk_o. ss. des_ifs; try reflexivity.
+        + right. ss. do 2 econs.
+        + right. ss. do 2 econs.
+      - clear. unfold mk_o. ss. des_ifs; try reflexivity.
+        + right. ss. do 2 econs.
+        + right. ss. do 2 econs.
+    }
+
+    { des. destruct GENOS0 as [GENOS IND]. eapply IH in IND; eauto.
+      guclo lsim_indC_spec. econs 16; eauto.
+      esplits; eauto.
+      clear - LT. unfold mk_o. des_ifs; try reflexivity.
+      - ss. do 2 econs. auto.
+      - ss. do 1 econs. auto.
+    }
+
+    { guclo lsim_indC_spec. econs 17; eauto. i.
+      specialize (GENOS _ _ _ _ _ _ _ INV0 VALID0 _ TGT). des.
+      destruct GENOS0 as [GENOS IND]. eapply IH in IND; eauto.
+      esplits; eauto.
+      clear - LT. unfold mk_o. des_ifs; try reflexivity.
+      - ss. do 2 econs. auto.
+      - ss. do 1 econs. auto.
+    }
+
+    { guclo lsim_indC_spec. econs 18; eauto. i.
+      specialize (GENOS _ _ _ _ _ _ _ INV0 VALID0 _ TGT). des.
+      destruct GENOS0 as [GENOS IND]. eapply IH in IND; eauto.
+    }
+
+    { eapply gensim_genos in GENOS. des.
+      guclo lsim_ord_weakLC_spec. econs.
+      guclo lsim_ord_weakRC_spec. econs.
+      instantiate (1:=mk_o (@wf_ot R0 R1) ot0 false src).
+      instantiate (1:=mk_o (@wf_ot R0 R1) os0 false tgt).
+      gfinal. right. pfold. eapply pind9_fold. econs 19. right. eapply CIH. auto.
+      - ss. des_ifs; try reflexivity. right. ss. do 2 econs.
+      - ss. des_ifs; try reflexivity. right. ss. do 2 econs.
+    }
+
+  Qed.
 
 End PROOF.
